core/effect_interpolation_II.v
@@ -4,16 +4,17 @@ Require Import Coqlib.
 Require Import Integers.
 Require Import compcert.common.Values.
 Require Import Maps.
-Require Import msl.Axioms.
+Require Import Axioms.
 
-Require Import FiniteMaps.
-Require Import sepcomp.StructuredInjections.
-Require Import sepcomp.reach.
+Require Import core.StructuredInjections.
+Require Import core.reach.
 Require Import effect_simulations.
 Require Import effect_simulations_lemmas.
-Require Import sepcomp.mem_lemmas.
-Require Import sepcomp.mem_interpolation_defs.
-Require Import sepcomp.mem_interpolation_II.
+Require Import core.mem_lemmas.
+Require Import core.mem_interpolation_defs.
+Require Import core.mem_interpolation_II.
+Require Import core.FiniteMaps.
+
 
 (*Inserts the new injection entries into extern component, but not into foreign*)
 Definition insert_as_extern (mu: SM_Injection) (j: meminj) (DomJ TgtJ:block->bool)
