core/effect_interpolation_proofs.v
@@ -1,6 +1,6 @@
-Require Import sepcomp.effect_interpolants.
-Require Import sepcomp.effect_interpolation_II.
-Require Import sepcomp.mem_interpolation_II.
+Require Import core.effect_interpolants.
+Require Import core.effect_interpolation_II.
+Require Import core.mem_interpolation_II.
 
 Module EffectInterpolations <: EffectInterpolationAxioms.
 Definition effect_interp_II := EFF_interp_II.
