core/effect_properties.v
@@ -5,17 +5,15 @@ Require Import compcert.common.Values.
 Require Import Maps.
 Require Import Integers.
 Require Import AST.
-
 Require Import Globalenvs.
+Require Import Axioms.
 
-Require Import msl.Axioms.
-
-Require Import sepcomp.mem_lemmas. (*needed for definition of mem_forward etc*)
-Require Import sepcomp.core_semantics.
-Require Import sepcomp.effect_semantics.
-Require Import sepcomp.StructuredInjections.
-Require Import sepcomp.reach.
-Require Import sepcomp.effect_simulations.
+Require Import core.mem_lemmas. (*needed for definition of mem_forward etc*)
+Require Import core.core_semantics.
+Require Import core.effect_semantics.
+Require Import core.StructuredInjections.
+Require Import core.reach.
+Require Import core.effect_simulations.
 
 Goal forall mu Etgt Esrc m2 m2' (WD: SM_wd mu) m1
             (TgtHyp: forall b ofs, Etgt b ofs = true -> 
@@ -1177,6 +1175,7 @@ Proof.
   (apply A; assumption) ||
   (eapply B; rewrite encode_int_length; congruence) || idtac.
 
+  eapply B. simpl in H. eassumption.
   eapply B. simpl in H. eassumption.
   eapply B. simpl in H. eassumption.
   eapply B. simpl in H. eassumption.
