core/effect_semantics.v
@@ -6,13 +6,12 @@ Require Import Maps.
 Require Import Integers.
 Require Import AST.
 Require Import Globalenvs.
+Require Import Axioms.
 
-Require Import msl.Axioms.
-Require Import sepcomp.mem_lemmas. (*needed for definition of mem_forward etc*)
-Require Import sepcomp.core_semantics.
-Require Import sepcomp.core_semantics_lemmas.
-Require Import sepcomp.StructuredInjections.
-
+Require Import core.mem_lemmas. (*needed for definition of mem_forward etc*)
+Require Import core.core_semantics.
+Require Import core.core_semantics_lemmas.
+Require Import core.StructuredInjections.
  
 Record EffectSem {G C} :=
   { sem :> CoopCoreSem G C;
