core/effect_simulationsEXP.v
@@ -12,11 +12,11 @@ Require Import compcert.common.Globalenvs.
 
 Require Import compcert.lib.Axioms.
 
-Require Import sepcomp.mem_lemmas. (*needed for definition of mem_forward etc*)
-Require Import sepcomp.core_semantics.
-Require Import sepcomp.effect_semantics.
-Require Import sepcomp.StructuredInjections.
-Require Import sepcomp.reach.
+Require Import core.mem_lemmas. (*needed for definition of mem_forward etc*)
+Require Import core.core_semantics.
+Require Import core.effect_semantics.
+Require Import core.StructuredInjections.
+Require Import core.reach.
 
 Module SM_simulation. Section SharedMemory_simulation_inject. 
 
