core/effect_simulations_lemmas.v
@@ -6,16 +6,15 @@ Require Import Maps.
 Require Import Integers.
 Require Import AST.
 Require Import Globalenvs.
+Require Import Axioms.
 
-Require Import msl.Axioms.
-Require Import sepcomp.mem_lemmas. (*needed for definition of mem_forward etc*)
-Require Import sepcomp.core_semantics.
-Require Import sepcomp.core_semantics_lemmas.
-Require Import sepcomp.effect_semantics.
-Require Import sepcomp.StructuredInjections.
-Require Import sepcomp.reach.
-
-Require Import effect_simulations.
+Require Import core.mem_lemmas. (*needed for definition of mem_forward etc*)
+Require Import core.core_semantics.
+Require Import core.core_semantics_lemmas.
+Require Import core.effect_semantics.
+Require Import core.StructuredInjections.
+Require Import core.reach.
+Require Import core.effect_simulations.
 
 Section Eff_INJ_SIMU_DIAGRAMS.
   Context {F1 V1 C1 F2 V2 C2:Type}
