core/rg_lemmas.v
@@ -5,17 +5,15 @@ Require Import compcert.common.Values.
 Require Import compcert.lib.Maps.
 Require Import compcert.lib.Integers.
 Require Import compcert.common.AST.
-
 Require Import compcert.common.Globalenvs.
-
 Require Import compcert.lib.Axioms.
 
-Require Import sepcomp.mem_lemmas. (*needed for definition of mem_forward etc*)
-Require Import sepcomp.core_semantics.
-Require Import sepcomp.effect_semantics.
-Require Import sepcomp.StructuredInjections.
-Require Import sepcomp.reach.
-Require Import sepcomp.effect_simulations.
+Require Import core.mem_lemmas. (*needed for definition of mem_forward etc*)
+Require Import core.core_semantics.
+Require Import core.effect_semantics.
+Require Import core.StructuredInjections.
+Require Import core.reach.
+Require Import core.effect_simulations.
 
 Definition FLIP mu := 
   match mu with
